common/dnf.lean
@@ -45,7 +45,7 @@ lemma dnf_prsv_pred [atom_type α β] (pr : α → Prop) :
     cases has with asp hasp, 
     cases hasp with hasp1 hasp2,
     cases asp with as1 as2, subst hasp2, 
-    cases (mem_or_mem_of_mem_append ha) with hm hm,
+    simp at ha, cases ha with hm hm,
     apply dnf_prsv_pred p hnmp as1,  
     apply fst_mem_of_mem_product hasp1, apply hm,  
     apply dnf_prsv_pred q hnmq as2, 
@@ -58,7 +58,8 @@ lemma dnf_prsv_pred [atom_type α β] (pr : α → Prop) :
     rewrite forall_mem_union at hnm,
     cases hnm with hnmp hnmq,
     unfold dnf, intros as has, intros a ha,
-    cases (mem_or_mem_of_mem_append has) with hm hm,
+    rewrite mem_append at has,
+    cases has with hm hm,
     apply dnf_prsv_pred p hnmp as hm a ha, 
     apply dnf_prsv_pred q hnmq as hm a ha 
   end
@@ -80,89 +81,66 @@ begin
   apply dnf_prsv_pred (normal β) _ hp, 
 end
 
-#check @mem_map_of_mem
-lemma dnf_prsv_alt [atom_type α β] : ∀ {p : fm α} {H : nqfree p} {xs : list β}, 
-  list.disj_list (list.map (allp (atom_type.val xs)) (dnf p)) ↔ I p xs 
-| (fm.true α) H bs := 
-  by {unfold dnf, simp, unfold disj_list, 
-      rewrite true_or, unfold I, unfold interp}
-| (fm.false α) H bs := 
-  by {unfold dnf, simp, unfold disj_list, rewrite exp_I_bot }
-| (fm.atom a) H bs := 
+lemma dnf_prsv [atom_type α β] : ∀ {p : fm α} {bs : list β},
+  nqfree p → (list.some_true (list.map (allp (atom_type.val bs)) (dnf p)) ↔ I p bs) 
+| (fm.true α) bs hf :=
   begin
-    unfold dnf, simp, unfold disj_list, simp, 
-    apply iff.intro, intro Ha, apply Ha, 
-    unfold I, unfold interp, apply id
+    unfold dnf, unfold map, unfold I,
+    unfold interp, simp, existsi true, simp
+  end 
+| (fm.false α) bs hf :=
+  begin
+    unfold dnf, unfold map, unfold I,
+    unfold interp, simp, intro hc, cases hc with p hp,
+    cases hp with hp1 hp2, cases hp1
+  end 
+| (fm.atom a) bs hf := 
+  begin
+    unfold dnf, unfold map, unfold I,
+    unfold interp, simp, unfold some_true,
+    apply iff.intro; intro h, cases h with p hp,
+    cases hp with hp1 hp2, rewrite mem_singleton at hp1,
+    subst hp1, apply hp2, existsi (val bs a), simp, apply h
   end
-| (fm.and p q) H bs := 
+| (p ∧' q) bs hf := 
   begin
-    unfold dnf, rewrite map_compose, rewrite exp_I_and, 
-    rewrite iff.symm (@dnf_prsv_alt p _ bs),
-    rewrite iff.symm (@dnf_prsv_alt q _ bs),
-    repeat {rewrite disj_list_iff_some_true},
-    repeat {unfold some_true},
-
-    apply iff.intro,
-    intro H0, cases H0 with r Hr, 
-    have Hrl := Hr^.elim_left,
-    have Hrr := Hr^.elim_right, clear Hr, 
-    cases (list.exists_of_mem_map Hrl) with d Hd,
-    simp at Hd, 
-    apply and.intro, 
-         
-    existsi (∀ (a : α), a ∈ (prod.fst d) → atom_type.val bs a),
-    cases Hd with hd1 hd2,
-    apply and.intro, 
-    rewrite iff.symm (allp_iff_forall_mem (val bs) d.fst), 
-    apply mem_map_of_mem,
+    cases hf with hfp hfq, unfold dnf,
+    unfold some_true, rewrite map_compose,
+    rewrite exp_I_and, 
+    rewrite iff.symm (@dnf_prsv p bs hfp),
+    rewrite iff.symm (@dnf_prsv q bs hfq),
+    apply iff.intro; intro h,
     
-    apply fst_mem_of_mem_product, apply hd1,
-    intros a Ha, subst hd2,
-    apply Hrr, cases d with dl dr, unfold append_pair,
-    apply mem_append_of_mem_or_mem,
-    apply or.inl Ha, 
+    cases h with r hr, cases hr with hr1 hr2,
+    rewrite mem_map at hr1, cases hr1 with ll hll,
+    cases hll with hll1 hll2, subst hll2, cases ll with lp lq,
+    unfold append_pair at hr2, rewrite mem_product at hll1,
+    cases hll1 with hlp hlq, unfold allp at hr2,
+    rewrite forall_mem_append at hr2, cases hr2 with hp hq,
+    apply and.intro,
+    existsi (allp (val bs) lp), 
+    apply and.intro (mem_map_of_mem _ hlp) hp,
+    existsi (allp (val bs) lq), 
+    apply and.intro (mem_map_of_mem _ hlq) hq,
 
-    existsi (∀ (a : α), a ∈ (prod.snd d) → atom_type.val bs a),
-    cases Hd with hd1 hd2,
-    apply and.intro, 
-    rewrite iff.symm (allp_iff_forall_mem (val bs) d.snd), 
-    apply mem_map_of_mem, 
-    apply snd_mem_of_mem_product hd1,
-    intros a Ha, subst hd2,
-    apply Hrr, cases d with dl dr, unfold append_pair,
-    apply mem_append_of_mem_or_mem,
-    apply or.inr Ha, 
-
-    intro H0, 
-    cases (H0^.elim_left) with r Hr,
-    cases (H0^.elim_right) with s Hs, clear H0, 
-    cases (list.exists_of_mem_map Hr^.elim_left) with ll Hll,
-    cases (list.exists_of_mem_map Hs^.elim_left) with lr Hlr,
-    existsi (∀ (a : α), a ∈ append_pair (ll,lr) → atom_type.val bs a),
-    apply and.intro, 
-    rewrite iff.symm (allp_iff_forall_mem (val bs) (append_pair (ll,lr))),
-    apply mem_map_of_mem _, 
-    apply mem_product_of_mem_and_mem,
-    apply Hll^.elim_left, apply Hlr^.elim_left,
-    intros a Ha, 
-    cases (mem_or_mem_of_mem_append Ha) with HM HM,
-    rewrite Hll^.elim_right at Hr,
-    apply Hr^.elim_right _ HM, 
-    rewrite Hlr^.elim_right at Hs,
-    apply Hs^.elim_right _ HM,
-    apply H^.elim_right, apply H^.elim_left
+    cases h with hp hq, 
+    cases hp with cp hcp, cases hcp with hcp1 hcp2, 
+    cases hq with cq hcq, cases hcq with hcq1 hcq2,
+    rewrite mem_map at hcp1, cases hcp1 with lp hlp,
+    cases hlp with hlp1 hlp2, subst hlp2,
+    rewrite mem_map at hcq1, cases hcq1 with lq hlq,
+    cases hlq with hlq1 hlq2, subst hlq2,
+    existsi (allp (val bs) (lp ++ lq)), apply and.intro,
+    rewrite mem_map, existsi (lp,lq), apply and.intro,
+    rewrite mem_product, apply and.intro; assumption,
+    refl, unfold allp, rewrite forall_mem_append,
+    apply and.intro hcp2 hcq2
   end
-| (fm.or p q) H bs := 
+| (p ∨' q) bs hf := 
   begin
-    unfold dnf, rewrite map_append, 
-    rewrite disj_list_dist_append,
-    rewrite dnf_prsv_alt, rewrite dnf_prsv_alt,
-    rewrite exp_I_or, apply H^.elim_right,
-    apply H^.elim_left
+    cases hf with hfp hfq,
+    unfold dnf, rewrite map_append, rewrite some_true_append,
+    rewrite @dnf_prsv p _ hfp, rewrite @dnf_prsv q _ hfq, rewrite exp_I_or,
   end
-| (fm.not p) H bs := by cases H
-| (fm.ex p) H bs := by cases H
-
-lemma dnf_prsv [atom_type α β] {p : fm α} {H : nqfree p} {bs : list β} : 
-  list.some_true (list.map (allp (atom_type.val bs)) (dnf p)) ↔ I p bs := 
-iff.trans (by rewrite some_true_iff_disj_list) (@dnf_prsv_alt _ _ _ _ H _)
+| (fm.not _) bs hf := by cases hf
+| (fm.ex _) bs hf := by cases hf
